*Matrices are a way of storing data in arrays. Adding or subtracting matrices of the same order, you compare each position and complete the function individually. Multiplying by a scalar quantity, you multiply each position by the quantity*

*Calc method for multiplication - `Math -> MAT/VCT -> Matrix Dimensions`*

The determinant of a matrix is important in a number of applications. The determinant of $\pmatrix{a&b\\c&d}=ad-bc$ *If there determinant is 0, then there is no way to undo the effects of it's transformation*

*Examples of matrix transformations where $(i, j)= \pmatrix{i_{1}&j_{1}\\i_{2}&j_{2}}$ :*
- $\pmatrix{-1&0\\0&-1}\to$  rotation of $180\degree$
- $\pmatrix{0&1\\1&0}\to$  reflection in $y=x$
- $\pmatrix{m&0\\0&m}\to$  enlargement by scale factor of $m$
- $\pmatrix{0&-1\\-1&0}\to$  reflection in $y=-x$
- $\pmatrix{\cos\theta&-\sin\theta\\\sin\theta&\cos\theta}\to$  anticlockwise rotation around origin by $\theta$
*For clockwise rotation you just take the negative and use the anticlockwise*

**Reflections on the line y=mx :**
$$y=(\tan\theta )x:\pmatrix{\cos2\theta&\sin2\theta\\\sin2\theta&-\cos2\theta}$$
*We can equate the gradient $\tan\theta$ to a new gradient m, derive a value for theta and use that theta value for the transformation*

*The transformation A followed by B is equal to the transformation of $B\cdot A$*

By multiplying $\pmatrix{x\\y\\1}$ by our transformation, we can gain a line of correct values in the cartesian plane. And if we're given a value for y in terms of x, we can substitute that line into our matrix, ie. $y=x+1\therefore\pmatrix{x\\y\\1}\to\pmatrix{x\\x+1\\1}$ 

**Non-linear transformations :**
*In linear transformations, the matrix are encoded to make the transformation from the origin, we achieve transformations around other points by introducing a z dimension pointer in our matrices.* In order to complete a multiplication with this new transformation matrix, you'll also need to add a z coord to your points. The following demonstrates this based on the origin point.$$\pmatrix{a&b\\c&d}\cdot\pmatrix{x\\y}\to\pmatrix{a&b&0\\c&d&0\\0&0&1}\cdot\pmatrix{x\\y\\1}$$
*And where $(p,q)$ represents the translation in $(x,y)$* $$\pmatrix{a&b\\c&d}\cdot\pmatrix{x\\y}\to\pmatrix{a&b&p\\c&d&q\\0&0&1}\cdot\pmatrix{x\\y\\1}$$
**3D Matrices Examples :**
- $\pmatrix{-1&0&0\\0&1&0\\0&0&1}$ represents a reflection against the x plane
- $\pmatrix{1&0&0\\0&\cos\theta&-\sin\theta\\0&\sin\theta&\cos\theta}$ anticlockwise rotation in x axis
- $\pmatrix{\cos\theta&0&\sin\theta\\0&1&0\\-\sin\theta&0&\cos\theta}$ anticlockwise rotation in y axis
- $\pmatrix{\cos\theta&-\sin\theta&0\\\sin\theta&\cos\theta&0\\0&0&1}$ anticlockwise rotation in z axis

**Inverse Matrices :**
An inverse matrix undoes the transformation, and so its a given that multiplying a matrix and it's inverse matrix products an identity matrix. The order of multiplication doesn't matter and the determinants multiplied = 1. Formula for a 2x2 inverse matrix:$$\text{inverse of }\pmatrix{a&b\\c&d}=\frac{1}{ad-bc}\pmatrix{d&-b\\-c&a}$$
**Proof by induction - Matrices to the power of n :**
*Using [[1.1 - Proof by Induction|Proof by Induction]] let's prove by induction that $\pmatrix{-2&-1\\9&4}^n=\pmatrix{1-3n&-n\\9n&3n+1}$*
$$\text{Let }P^{n}=\pmatrix{-2&-1\\9&4}^n=\pmatrix{1-3n&-n\\9n&3n+1}$$
*Let's first prove this works for it's minimum valid integer*
$$\text{Let }n=1\to\pmatrix{-2&-1\\9&4}^{1}=\pmatrix{1-3(1)&-(1)\\9(1)&3(1)+1}=\pmatrix{1-3&-1\\9&3+1}=\pmatrix{-2&-1\\9&4}$$
*Now that we've proved that n=1 gives a valid solution, let's work some induction magic and prove that for all valid values n, n+1 also gives valid solution. It's important to note what we're working towards, ie. $\pmatrix{1-3(n+1)&-(n+1)\\9(n+1)&3(n+1)+1}$*
$$P^{n}\cdot P=P^{n+1}\to\pmatrix{1-3n&-n\\9n&3n+1}\cdot\pmatrix{-2&-1\\9&4}=\pmatrix{-9n+6n-2&-4n-1+3n\\27n+9-18n&12n+4-9n}$$
*And finally with a bit of rearranging, we can get to :*
$$=\pmatrix{1-3n-3&-n-1\\9n+9&3n+4}=\pmatrix{1-3(n+1)&-(n+1)\\9(n+1)&3(n+1)+1}=P^{n+1}$$
*If it is true for $P^{n}$, it is true for $P^{n+1}$. Since it is true for $n=1$, it's then true for all positive integers larger than $1$ - proven by proof by induction*