**Method :**
$$\text{Assume }\frac{f_1(x)}{f_2(x)}\equiv\frac{f_1(x)}{CD}\equiv\frac{A}{C}+\frac{B}{D}\equiv\frac{AD+BC}{CD}\therefore f_1(x)\equiv AD+BC$$ Form *simultaneous equations*, defining $x$ where $C = 0$ and where $D = 0$ allowing us to define the values of $A$ and $B$.

**Altered Method with a squared 'D' :**
$$\text{Assume }\frac{f_1(x)}{f_2(x)}\equiv\frac{f_1(x)}{CD^{2}}\equiv\frac{A}{C}+\frac{B}{D^{2}}+\frac{E}{D}\equiv\frac{AD^{2}+BC+ECD}{CD^{2}}$$$$\therefore f(x)\equiv AD^{2}+BC+ECD$$Form *simultaneous equations*, defining $x$ where $C = 0$ and where $D^{2} = 0$ allowing us to define the values of $A$ and $B$. Now we need to find the valued of $E$

We must now *equate the coefficients* of $x^{2}$ 