From the hyperbolic function $x^{2}-y^{2}=1$ we derive $\cosh A$ and $\sinh A$, [refer to graph](https://ds055uzetaobb.cloudfront.net/brioche/uploads/fD7jZptgCQ-hyperbolic-functions.png)

**The Original Definitions**
$$\sinh x=\frac{e^{x}-e^{-x}}{2}\hspace{1cm}\cosh x=\frac{e^{x}+e^{-x}}{2}\hspace{1cm}\tanh x =\frac{\sin x}{\cos x}=\frac{e^{x}-e^{-x}}{e^{x}+e^{-x}}=\frac{e^{2x}-1}{e^{2x}+1}$$
[Cosh x Diagram](https://www.medcalc.org/manual/functions/cosh.png) and [Sinh x Diagram](https://www.medcalc.org/manual/functions/sinh.png)

**Deriving Identities :**
$$\cosh^{2} x-\sinh^{2} x=1\hspace{1cm}\cosh^{2} x+\sinh^{2} x=\cosh 2x\hspace{1cm}2\sinh A\cosh A=\sinh 2A$$
*And double angle*
$$\sinh (A\pm B)=\sinh A\cosh B\pm \cosh A\sinh B\hspace{0.5cm}\cosh (A\pm B)=\cosh A\cosh B\pm \sinh A\sinh B$$
*Defining tanh 2x*
$$\tanh 2x=\frac{\sinh 2x}{\cosh 2x}=\frac{2\sinh x\cosh x}{(\cosh x)^{2}+(\sinh x)^{2}}=\frac{2\tanh x}{1+(\tanh x)^2}$$
**Identities derived from Hyperbolic Function**
- $1-(\tanh x)^{2}=(\sec h x)^{2}$
- $(\cot h x)^{2}-1=(\csc h x)^{2}$ 

**Defining Inverse Hyperbolic functions**
Recall from Math Unit 3 how to define an inverse function, we set y = to the inverse function, apply the function to both sides and rearrange for y.

Additional subtopics:
```folder-index-content
```