**A) Show that $(2+e^{i\theta})(2+e^{-i\theta})=5+4\cos\theta$**
$$(2+e^{i\theta})(2+e^{-i\theta})=4+2e^{i\theta}+2e^{-i\theta}+1=5+2(e^{i\theta}+e^{-i\theta})=5+4\cos\theta$$
**B) Find the value of S**
$$C-iS = 1-\frac{\cos\theta}{2}+\frac{\cos2\theta}{2^{2}}-\frac{\cos3\theta}{2^{3}}+...-i(\frac{\sin\theta}{2}-\frac{\sin2\theta}{2^{2}}+\frac{\sin3\theta}{3^{3}}-...)$$
Collect terms together
$$C-iS = 1-\frac{\cos\theta+i\sin\theta}{2}+(\frac{\cos\theta+i\sin\theta}{2})^{2}-(\frac{\cos\theta+i\sin\theta}{2})^{3}+...$$
Sub in the identity $e^{i\theta}=\cos\theta+i\sin\theta$
$$C-iS = 1-\frac{e^{i\theta}}{2}+(\frac{-e^{i\theta}}{2})^{2}+(\frac{-e^{i\theta}}{2})^{3}+...\hspace{1cm}\text{This is a geometric series : } a=1, r=-\frac{e^{i\theta}}{2}$$
Use the sum to infinity of [[Geometric]] Series.
$$C-iS =S_\infty=\frac{1}{1--\frac{e^{i\theta}}{2}}=\frac{2}{2+e^{i\theta}}$$
Use solution **Part A** to simplify this equation, multiply top and bottom by $2+e^{-i\theta}$
$$C-iS ==\frac{2(2+e^{-i\theta})}{(2+e^{i\theta})(2+e^{-i\theta})}=\frac{4+2e^{-i\theta}}{5+4\cos\theta}=\frac{4+2\cos\theta-2i\sin\theta}{5+4\cos\theta}$$
Finally equate imaginary terms 
$$-S=\frac{-2\sin\theta}{5+4\cos\theta}\implies S=\frac{2\sin\theta}{5+4\cos\theta}$$
