**Note that conjugate pairs only appear for roots of real numbers**

**Finding $\sqrt{i}$ using [[De Moivre's Theorem]]**
$$Z=r(\cos\theta+i\sin\theta)$$
By evaluating the argument and modulus of i, we find the following
$$i=1(\cos\frac{\pi}{2}+\sin\frac{\pi}{2})\implies \pm i^{\frac{1}{2}}=\pm(\cos\frac{\pi}{2}+\sin\frac{\pi}{2})^{\frac{1}{2}}$$
[[De Moivre's Theorem]] identities allow us to turn that into the following
$$\pm i^{\frac{1}{2}}=\pm(\cos\frac{\pi}{4}+\sin\frac{\pi}{4})=\frac{1+i}{\sqrt{2}}\text{ or }\frac{-1-i}{\sqrt{2}}$$
**Defining $e^{i\theta}$ as an alternative for for complex numbers**
Recall the following Maclaurin's and Taylor's Series Identities :
$$\sin x=x-\frac{x^{3}}{3!}+\frac{x^{5}}{5!}-...+(-1)^{r+1}\frac{x^{2r+1}}{(2r+1)!}+...$$
$$\cos x=1-\frac{x^{2}}{2!}+\frac{x^{4}}{4!}-...+(-1)^{r}\frac{x^{2r}}{(2r)!}+...$$
$$e^{x}=1+x+\frac{x^{2}}{2!}+...+\frac{x^{r}}{r!}+...$$
Now onto the proof, Let $x=i\theta$
$$e^{i\theta}=1+i\theta+\frac{(i\theta)^{2}}{2!}+\frac{(i\theta)^{3}}{3!}+\frac{(i\theta)^{4}}{4!}+...=1+i\theta-\frac{\theta^{2}}{2!}-\frac{i\theta^{3}}{3!}+\frac{\theta^{4}}{4!}+...$$
By collecting real and imaginary components, we get the following
$$e^{i\theta}=+...=(1-\frac{\theta^{2}}{2!}+\frac{\theta^{4}}{4!}+...)+i(\theta-\frac{\theta^{3}}{3!}+...)=\cos\theta+i\sin\theta$$
Therefore, where the r is 0, $e^{i\theta}$ can represent a complex number.

Additional subtopics:
```folder-index-content
```