The gradient function or derivative of the curve $y=f(x)$ is written as $f'(x)$ $or \frac{dy}{dx}$

To calculate the gradient between two points, we can use the formula : $$\frac{y_1-y_2}{x_1-x_{2}} \text{ which we could represent as :} \frac{f(x_1)-f(x_2)}{x_1-x_{2}}$$
Using this formula for the coordinates $(x,f(x))$ and $(x+h,f(x+h))$, we get :
$$y=\frac{f(x+h)-f(x)}{x+h-x}$$
Consider that the closer the coordinate $(x+h,f(x+h))$ is to $(x,f(x))$, the closer we are to the gradient of just $(x,f(x))$. 
We can represent this with $\lim_{h\to0}$, where h (the difference) tends towards zero
$$f'(x)=\lim_{h\to 0}\frac{f(x+h)-f(x)}{h}$$
Once we have simplified the fraction, we can disregard any $+h$ as $h$ has tended to 0. This gives us out gradient at the point $(x, f(x))$

*Power Rule ~ The Cheat Method*
Where $a\text{, }b\text{ and }c$ are constants
$$
y=ax^{n}+bx^1+c... \to\frac{dy}{dx} = anx^{n-1}+b...
$$


Additional subtopics:
```folder-index-content
```