When completing the square, this is the easiest method to calculating $x$
*First we factor out the coefficient of $x^{2}$* 
$$ax^{2}+bx+c = a(x^2+\frac{bx}{a})+c$$
*We then bring the c to other side*
$$a(x^2+\frac{bx}{a})=-c$$
*We then have to force the quadratic into a repeated root*
$$(x^2+\frac{bx}{a})=(x+\frac{b}{2a})^2-(\frac{b}{2a})^2$$
*Plug that back into the formula*
$$a((x+\frac{b}{2a})^2-(\frac{b}{2a})^2)=-c$$
*Let's isolate that repeated root*
$$(x+\frac{b}{2a})^2=(\frac{b}{2a})^2-\frac{c}{a}$$
*Then square root*
$$x+\frac{b}{2a}=\pm\sqrt{(\frac{b}{2a})^2-\frac{c}{a}}$$
*Rearrange to isolate the x term*
$$x=-\frac{b}{2a}\pm\sqrt{\frac{b^2}{4a^2}-\frac{c}{a}}$$
*Voila, with a bit of rearranging...
$$x=-\frac{b}{2a}\pm\sqrt{\frac{b^2}{4a^2}-\frac{4ac}{4a^2}}$$
*... you've just discovered the quadratic formula**
$$x=\frac{-b\pm\sqrt{b^2-4ac}}{2a}$$
