This shifts the curve $-a$ on the $x$ axis : $y=(x+a)^2$
This shifts the curve $a$ on the $y$ axis : $y=x^2+a$ 

Setting $y=0$ allows us to calculate the coordinates that the curve crosses the $x$ axis, this is done by factorising the equation $y=ax^2+bx+c$

Setting $x=0$ allows us to calculate the coordinates that the curve crosses the $y$ axis, using $y=ax^2+bx+c$, by set $x=0$, that means that $y=a(0)^2+b(0)+c, y=c$

Using [[Completing the Square]] , we can rearrange the equation in this format : $y=(x+a)^2+b$, we can use this to calculate the minimum point of the curve as $(-a,b)$

*Remember we can always work backwards and turn these equations back into its original quadratic equation*