$$\text{let }b^{y}=x\text{, }\log_bx=y$$
**Log rules :**
- $\log_a1=0$
- $\text{When }b\leq0\text{, }\log_{a}b\text{ is undefined}$
- $\log_{a}a=1$
- $\log_{a}\frac{1}{a}=-1$
- $\log_{e}x=\ln x$
- $\log_{10}x=\log x$

**Log Laws :**
$$\log_{a}b+\log_{a}c=\log_x(bc)$$ *Proof :*
$\text{Let }x=\log_{a}b\rightarrow a^{x}=b$
$\text{Let }y=\log_{a}c\rightarrow a^{y}=c$
$bc = a^{x}\cdot a^{y}=a^{x+y}$
$\log_{a}bc=x+y$
$\log_{a}bc=\log_{a}b+\log_{a}c$
$$\log_{a}b-\log_{a}c=\log_x(\frac{b}{c})$$ *Proof :*
$\text{Let }x=\log_{a}b\rightarrow a^{x}=b$
$\text{Let }y=\log_{a}c\rightarrow a^{y}=c$
$\frac{b}{c} = a^{x}\divsymbol a^{y}=a^{x-y}$
$\log_{a}\frac{b}{c}=x-y$
$\log_{a}\frac{b}{c}=\log_{a}b-\log_{a}c$
$$\log_{a}b^{n}=n\log_{a}b$$
 *Proof :*
$\text{Let }x=\log_{a}b^{n}\rightarrow a^{x}=b^{n}$
$a^{x}=b^{n}\rightarrow a^{\frac{x}{n}}=b$
$\frac{x}{n}=\log_{a}b$
$x=n\log_{a}b$
$\log_{a}b^{n}=n\log_{a}b$
